Cool, our two definitions of contraction are equivalent

src/graph_theory/contraction.lean
@@ -68,10 +68,10 @@ namespace simple_graph
     def is_contraction (G : simple_graph V) (G' : simple_graph V') : Prop
         := ∃ S : contraction.setup G', nonempty (G ≃g (G'/S))
 
-    def is_contraction' (G : simple_graph V) (G' : simple_graph V') : Prop
+    def is_surjective_push (G : simple_graph V) (G' : simple_graph V') : Prop
         := ∃ φ : V' -> V, surjective φ ∧ G = push φ G'
 
-    example : (∃ S : setoid V', nonempty (G ≃g G'/S)) <-> is_contraction' G G' :=
+    example : (∃ S : setoid V', nonempty (G ≃g G'/S)) <-> is_surjective_push G G' :=
     begin
         split,
         { rintro ⟨S,⟨⟨f,f',h₁,h₂⟩,h₃⟩⟩,
@@ -115,6 +115,70 @@ namespace simple_graph
             let := select.push_walk p hp, apply linked.linked_iff.mpr, use this },
         { rintros h₁ x y h₂, specialize h₁ (f y) ⟨x,h₂⟩ ⟨y,rfl⟩, replace h₁ := linked.linked_iff.mp h₁,
             cases h₁ with p, let := select.pull_walk p, use this, exact select.pull_walk_spec p }
+    end
+
+    def is_contraction' (G : simple_graph V) (G' : simple_graph V') : Prop
+        := ∃ φ : V' -> V, surjective φ ∧ adapted φ G' ∧ G = push φ G'
+
+    example : is_contraction G G' ↔ is_contraction' G G' :=
+    begin
+        split,
+        { rintro ⟨S,⟨⟨f,f',h₁,h₂⟩,h₃⟩⟩, simp [contraction] at h₃, let φ : V' -> V := f' ∘ quotient.mk', refine ⟨φ,_,_,_⟩,
+            { exact (left_inverse.right_inverse h₁).surjective.comp quotient.surjective_quotient_mk' },
+            { rw adapted_iff, intro z, intros x y, rcases x with ⟨x,hx⟩, rcases y with ⟨y,rfl⟩, simp [φ] at hx,
+                replace hx := h₂.left_inverse.injective hx, replace hx := quotient.eq.mp hx,
+                replace hx := linked.linked_iff.mp hx, cases hx with p,
+                suffices : ∀ z ∈ p.support, φ z = φ y, by {
+                    apply linked.linked_of_subgraph (select.mono S.sub),
+                    apply linked.linked_iff.mpr,
+                    use select.push_walk p this },
+                induction p with a a b c hi p ih,
+                { intros z h, cases h, rw h, cases h },
+                { intros z h, cases h, rwa h, suffices : φ a = φ b, rw this at hx, exact ih hx z h,
+                    simp [φ], apply congr_arg, apply quotient.eq.mpr, apply linked.step, exact hi }
+            },
+            { ext a b, rw <-h₃, split,
+                { rintros ⟨p₁,x,y,p₂,p₃,p₄⟩, refine ⟨ne_of_apply_ne f p₁,x,y,_,_,p₄⟩,
+                    convert congr_arg f' p₂, rw h₁, convert congr_arg f' p₃, rw h₁, },
+                { rintros ⟨p₁,x,y,rfl,rfl,p₂⟩, refine ⟨h₁.injective.ne p₁,x,y,_,_,p₂⟩,
+                    simp [φ], rw h₂, refl, simp [φ], rw h₂, refl } }
+        },
+        { rintro ⟨f,h₁,h₂,h₃⟩, subst h₃,
+            let g : simple_graph V' := {
+                adj := λ x' y', f x' = f y' ∧ G'.adj x' y',
+                symm := λ x' y' ⟨h₁,h₂⟩, ⟨h₁.symm,h₂.symm⟩,
+                loopless := λ x' ⟨h₁,h₂⟩, G'.ne_of_adj h₂ rfl },
+            let S : contraction.setup G' := ⟨g, λ x' y' h, h.2⟩, use S, letI : setoid V' := S.setoid,
+            let preimage : V → V' := λ x, classical.some (h₁ x),
+            have p₂ : ∀ x, f (preimage x) = x := λ x, classical.some_spec (h₁ x),
+            let F : V → S.clusters := λ x, ⟦preimage x⟧,
+            let F' : S.clusters → V := λ x, f x.out,
+            have p₃ : ∀ {x y}, S.g.linked x y ↔ f x = f y := by {
+                intros x y, split,
+                { intro h, induction h with a b h₁ h₂ h₃, refl, exact h₃.trans h₂.1 },
+                { intro h, specialize h₂ x y h, cases h₂ with p hp, apply linked.linked_iff.mpr, refine ⟨_⟩,
+                    induction p with a a b c h₃ p ih, refl,
+                    have h₄ : f b = f c := by { apply hp, right, apply walk.start_mem_support },
+                    refine walk.cons ⟨h.trans h₄.symm,h₃⟩ _, apply ih h₄, intros z hz, apply hp, right, exact hz }
+            },
+            have H₁ : left_inverse F' F := by {
+                intro x, simp [F',F], refine eq.trans _ (p₂ x), apply p₃.mp,
+                change ⟦preimage x⟧.out ≈ (preimage x), apply quotient.eq.mp, simp },
+            have H₂ : right_inverse F' F := by {
+                intro x', simp [F',F], refine eq.trans _ (quotient.out_eq _),
+                apply quotient.eq.mpr, apply p₃.mpr, apply p₂ },
+            refine ⟨⟨⟨F,F',H₁,H₂⟩,_⟩⟩,
+            simp [push,contraction,contraction.setup.setoid,quotient_graph,F], intros a b, split,
+            { rintros ⟨h₁,x,h₂,y,h₃,h₄⟩, refine ⟨_,x,_,y,_,h₄⟩,
+                { intro h, rw h at h₁, contradiction },
+                { rw ←p₂ a, apply p₃.mp, exact quotient.eq.mp h₂ },
+                { rw ←p₂ b, apply p₃.mp, exact quotient.eq.mp h₃ } },
+            { rintros ⟨h₁,x,rfl,y,rfl,h₂⟩, refine ⟨_,x,_,y,_,h₂⟩,
+                { intro h, have := quotient.eq.mp h, have := p₃.mp this, rw [p₂ _,p₂ _] at this, exact h₁ this },
+                { apply quotient.eq.mpr, apply p₃.mpr, rw p₂ _ },
+                { apply quotient.eq.mpr, apply p₃.mpr, rw p₂ _ },
+            }
+        }
     end
 
     infix ` ≼c `:50 := is_contraction
